tlc/assert/term.v
@@ -11,24 +11,24 @@ Unset Printing Implicit Defensive.
 
 (* Typed terms representing variables, constants, and applications *)
 Inductive term {C} : type -> Type :=
-| Flexible (x : flexible_var) : term (type_flexible_var x)
+| Flexible {t} (x : @flexible_var C t) : term t
 | Rigid {t} (x : @rigid_var C t) : term t
 | Const {t} (c : @denote_type C t) : term t
 | App {d r} (f : term (d -> r)) (x : term d) : term r.
 
+Coercion Flexible : flexible_var >-> term.
 Coercion Rigid : rigid_var >-> term.
 
 Bind Scope tlc_core_scope with term.
 
 (* Notations for constructing terms *)
-Notation "f <- x" :=
-  (App f x)
+Notation "f <- x" := (App f x)
   (at level 10, left associativity) : tlc_core_scope.
 
 (* Extracts the types of rigid variable used in a term *)
 Fixpoint term_var_types {C te} (e : @term C te) :=
   match e with
-  | Flexible _ => [::]
+  | Flexible _ _ => [::]
   | Rigid t _ => [:: t]
   | Const _ _ => [::]
   | App _ _ f x => undup (term_var_types f ++ term_var_types x)
@@ -37,7 +37,7 @@ Fixpoint term_var_types {C te} (e : @term C te) :=
 (* Extracts the rigid variables used in a term *)
 Fixpoint term_vars {C te} (e : @term C te) (t : type) : seq (@rigid_var C t) :=
   match e with
-  | Flexible _ => [::]
+  | Flexible _ _ => [::]
   | Rigid t' x =>
     if t' == t then
       let: n := unwrap_rigid_var x in
@@ -55,7 +55,7 @@ Fixpoint term_subst {C te} (s : forall t, @substitution C t) (e : @term C te)
 : @term C te.
   inversion e.
   - (* Flexible *)
-    rewrite H; by assumption.
+    by assumption.
   - (* Rigid *)
     specialize (s _ x); case s => [e' | ]; by assumption.
   - (* Const *)
